feat: Min/Max typeclasses

tests/lean/run/1025.lean
@@ -2,6 +2,10 @@ inductive Vector (α : Type u): Nat → Type u where
 | nil : Vector α 0
 | cons (head : α) (tail : Vector α n) : Vector α (n+1)
 
+class Order (α : Type u) extends LE α, LT α, Max α where
+  ltDecidable : DecidableRel (@LT.lt α _)
+  max_def x y : max x y = if x < y then x else y
+
 namespace Vector
   def mem (a : α) : Vector α n → Prop
   | nil => False
@@ -11,10 +15,10 @@ namespace Vector
   | nil     => init
   | cons a l => f a (foldr f init l)
 
-  theorem foldr_max [LE β] [LT β] [DecidableRel (· < · : β → β → Prop)] {v: Vector α n} (f : α → β) (init : β)
+  theorem foldr_max [Order β] {v: Vector α n} (f : α → β) (init : β)
     (h: v.mem y):
     f y ≤ v.foldr (λ x acc => max (f x) acc) init := by
-    induction v <;> simp only[foldr,max]
+    induction v <;> simp only[foldr,Order.max_def]
     · admit
     · split <;> admit
 end Vector
